

## Series $n^\circ 2$ -Numerical Sequences-

### Generalities

**Exercise 1.** Comment if the following statements are true or false? And give a valid reason for saying so.

- Every bounded sequence is convergent. **False**

**Counterexample.** Let  $u_n = (-1)^n$  be a bounded sequence such that  $|(-1)^n| \leq 1$ , but

$$\lim_{n \rightarrow +\infty} (-1)^n = \begin{cases} 1 & \text{if } n = 2k, \\ -1 & \text{if } n = 2k + 1. \end{cases}$$

does not exist. Then  $((-1)^n)_n$  D.V.

- Every sequence  $(u_n)_n$  satisfies  $u_{n+1} \leq u_n$  is decreasing. **False**

**Counterexample.** Let  $u_n = (-1)^n$ , we have  $u_1 < u_2$ , but the sequence  $(-1)^n$  is not decreasing.

- The sum of two divergent sequences is a divergent sequence. **False**

**Counterexample.** Let  $u_n = (-1)^n$  and  $v_n = (-1)^{n+1}$  be two divergent sequences, but

$$\lim_{n \rightarrow +\infty} (u_n + v_n) = \lim_{n \rightarrow +\infty} (-1)^n + (-1)^{n+1} = 0 \quad \text{C.V.}$$

- The product of two divergent sequences is a divergent sequence. **False**

**Counterexample.** Let  $u_n = (-1)^n$  and  $v_n = (-1)^{n+1}$  be two divergent sequences, but

$$\lim_{n \rightarrow +\infty} u_n v_n = \lim_{n \rightarrow +\infty} (-1)^{2n+1} = -1 \quad \text{C.V.}$$

- If the sequence  $(u_n)_{n \in \mathbb{N}}$  is increasing and  $u_n \leq n$ , then  $(u_n)_n$  is convergent. **False**

**Counterexample.** Let  $u_n = \sqrt{n}$  be an increasing sequence and  $\sqrt{n} \leq n$ , but  $(u_n)_n$  is divergent.

- If  $\lim_{n \rightarrow +\infty} u_n^2 = \ell^2$ , then  $\lim_{n \rightarrow +\infty} u_n = \ell$ . **False**

**Counterexample.** Let  $u_n = (-1)^n$ , we have

$$\lim_{n \rightarrow +\infty} u_n^2 = \lim_{n \rightarrow +\infty} (-1)^{2n} = 1 \not\Rightarrow \lim_{n \rightarrow +\infty} u_n = \lim_{n \rightarrow +\infty} (-1)^n = 1,$$

because  $\lim_{n \rightarrow +\infty} (-1)^n$  does not exist.

- If  $\lim_{n \rightarrow +\infty} |u_n| = |\ell|$ , then  $\lim_{n \rightarrow +\infty} u_n = \ell$ . **False**

**Counterexample.** Let  $u_n = (-1)^n$ , we have  $|u_n| \rightarrow 1$ , but according to our knowledge  $(-1)^n$  D.V.

### Convergent Sequences

**Exercise 2.** I) Consider the real sequence  $(u_n)_{n \in \mathbb{N}^*}$  defined as:  $u_n = \frac{n+1}{2n}$ .

$$(u_n)_n \text{ converges to } \ell \iff (\forall \varepsilon > 0, \exists n_0 \in \mathbb{N}, \forall n \in \mathbb{N}; n \geq n_0 \Rightarrow |u_n - \ell| < \varepsilon).$$

Find the absolute value of this inequality  $0.49 < u_n < 0.51$ , then deduce  $\ell, \varepsilon$  and  $n_0$ .

we can write the interval as absolute value,

$$\text{if } a < x < b \iff |x - x_0| < r_0, \text{ such that } x_0 = \frac{a+b}{2}, \text{ and } r_0 = \frac{b-a}{2}.$$

So,  $x_0 = \frac{0.49 + 0.51}{2} = \frac{1}{2}$  and  $r_0 = \frac{0.51 - 0.49}{2} = \frac{1}{10^2}$ .

Therefore,  $|u_n - \frac{1}{2}| < 10^{-2}$ , we conclude that  $\ell = \frac{1}{2}$ ,  $\varepsilon = 10^{-2}$ .

Applying the above definition, we get

$$|u_n - \frac{1}{2}| = \left| \frac{n+1}{2n} - \frac{1}{2} \right| = \frac{1}{2n} < 10^{-2}$$

$$\Rightarrow 2n > 100 \Rightarrow n > 50.$$

Then, its enough to take  $n_0 = [50] + 1 = 51$ .

► Use the previous definition to prove each of the following:

- $\lim_{n \rightarrow +\infty} \frac{2 \ln(n+1)}{\ln(n)} = 2$ . Using the definition, we have

$$\forall \varepsilon > 0, \exists n_0 \in \mathbb{N}, \forall n \in \mathbb{N}; n \geq n_0 \Rightarrow \left| \frac{2 \ln(n+1)}{\ln(n)} - 2 \right| < \varepsilon$$

$$\left| \frac{2 \ln(n+1)}{\ln(n)} - 2 \right| = \left| \frac{2 \ln(n+1) - 2 \ln(n)}{\ln(n)} \right|$$

$$= \frac{2 \ln\left(\frac{n+1}{n}\right)}{\ln(n)} \leq \frac{2 \ln(2)}{\ln(n)}$$

Since,  $1 + \frac{1}{n} \leq 2 \Rightarrow \ln(1 + \frac{1}{n}) \leq \ln(2)$ . Solving for  $n$  is now easy

$$\frac{2 \ln(2)}{\ln(n)} < \varepsilon \Leftrightarrow \ln(n) > \frac{\ln(4)}{\varepsilon} \Leftrightarrow n > \exp\left(\frac{\ln(4)}{\varepsilon}\right)$$

Then, it's enough to take  $n_0 = \left\lceil \exp\left(\frac{\ln(4)}{\varepsilon}\right) \right\rceil + 1 \in \mathbb{N}^*$ .

- $\lim_{n \rightarrow +\infty} \frac{5n+3}{7n+1} = \frac{5}{7}$ . Using the definition, we have

$$\forall \varepsilon > 0, \exists n_0 \in \mathbb{N}, \forall n \in \mathbb{N}; n \geq n_0 \Rightarrow \left| \frac{5n+3}{7n+1} - \frac{5}{7} \right| < \varepsilon$$

$$\left| \frac{5n+3}{7n+1} - \frac{5}{7} \right| = \left| \frac{16}{49n+7} \right| = \frac{16}{49n+7}$$

Solving for  $n$  is now easy

$$\frac{16}{49n+7} < \varepsilon \Leftrightarrow \frac{16}{\varepsilon} < 49n+7 \Leftrightarrow n > \frac{16-7\varepsilon}{49\varepsilon}.$$

Then, its enough to take  $n_0 = \left\lceil \frac{16-7\varepsilon}{49\varepsilon} \right\rceil + 1 \in \mathbb{N}$ .

**II) Study the convergence of the following sequences:**

**1)**  $u_n = \frac{\sin(n)}{n}$ .

Let  $v_n = \sin(n)$  is bounded, because  $|\sin(n)| \leq 1$ , and  $w_n = \frac{1}{n} \xrightarrow{n \rightarrow +\infty} 0$ .

Moreover,  $(u_n)_n$  is the product of two sequences, one of them is bounded and the other is convergent to zero. Then,  $(u_n)$  converges to zero.

**2)**  $u_n = \frac{1}{n^3} \sum_{k=1}^n k$ ,  $n \in \mathbb{N}^*$ .

We notice that the numerator is a sum of an arithmetic sequence, so

$$\sum_{k=1}^n k = 1 + 2 + 3 + \dots + n = \frac{n(n+1)}{2}$$

Therefore,  $u_n = \frac{n(n+1)}{2} \times \frac{1}{n^3} \xrightarrow{n \rightarrow +\infty} 0$ .

Then,  $(u_n)_n$  is convergent to 0.

- 3)  $u_n = \sum_{k=1}^n \frac{1}{\sqrt{n^2 + k}}$ .  
For every  $n \in \mathbb{N}^*$ , we have

$$\begin{aligned} 1 &\leq \frac{k}{n^2 + 1} \leq \frac{n}{n^2 + n} \\ \frac{1}{\sqrt{n^2 + 1}} &\leq \frac{1}{\sqrt{n^2 + k}} \leq \frac{1}{\sqrt{n^2 + n}} \\ \sum_{k=1}^n \frac{1}{\sqrt{n^2 + k}} &\leq u_n \leq \sum_{k=1}^n \frac{1}{\sqrt{n^2 + 1}} \\ \frac{1}{\sqrt{n^2 + n}} &\leq u_n \leq \frac{1}{\sqrt{n^2 + 1}} \\ \lim_{n \rightarrow +\infty} \frac{1}{n\sqrt{1 + 1/n}} &\leq \lim_{n \rightarrow +\infty} u_n \leq \lim_{n \rightarrow +\infty} \frac{1}{n\sqrt{1 + 1/n}} \\ 1 &\leq \lim_{n \rightarrow +\infty} u_n \leq 1. \end{aligned}$$

Then, by squeeze theorem, the sequence  $(u_n)_n$  converges to 1.

- 4)  $u_n = \frac{3^n - 7^n}{3^n + 7^n}$ . We have

$$\lim_{n \rightarrow +\infty} u_n = \lim_{n \rightarrow +\infty} \frac{\left(\frac{3}{7}\right)^n - 1}{\left(\frac{3}{7}\right)^n + 1} = -1.$$

Since,  $\left(\frac{3}{7}\right)^n$  is a geometric sequence of reason  $\left(\frac{3}{7}\right) < 1$ , then  $\left(\frac{3}{7}\right)^n \xrightarrow[n \rightarrow +\infty]{} 0$ .

Therefore,  $(u_n)_n$  converges to  $-1$ .

- 5)  $u_n = \frac{1}{n^2} \sum_{k=1}^n [kx]$ ,  $n \in \mathbb{N}^*$ , we have

$$\begin{aligned} x - 1 &< [x] \leq x \\ 2x - 1 &< [2x] \leq 2x \\ 3x - 1 &< [3x] \leq 3x \\ &\vdots \\ nx - 1 &< [nx] \leq nx \end{aligned}$$

By adding all sides, we find

$$\begin{aligned} (x - 1) + (2x - 1) + \cdots + nx - 1 &< [x] + [2x] + \cdots + [nx] \leq x + 2x + \cdots + nx \\ \frac{1}{n^2} [x(1 + 2 + \cdots + n) + (1 + 1 + \cdots + 1)] &< u_n \leq \frac{1}{n^2} [x(1 + 2 + \cdots + n)] \\ \frac{nx(n+1)}{2n^2} - \frac{n}{n^2} &< u_n \leq \frac{nx(n+1)}{2n^2} \\ \lim_{n \rightarrow +\infty} \left[ \frac{nx(n+1)}{2n^2} - \frac{n}{n^2} \right] &< \lim_{n \rightarrow +\infty} u_n \leq \lim_{n \rightarrow +\infty} \frac{nx(n+1)}{2n^2} \\ x/2 &< \lim_{n \rightarrow +\infty} u_n \leq x/2. \end{aligned}$$

Then by squeeze theorem, the sequence  $(u_n)_n$  converges to  $x/2$ .

- 6)  $u_n = \sqrt[3]{1+n} - \sqrt[3]{n}$ .

We have

$$a^3 - b^3 = (a - b)(a^2 + ab + b^2).$$

Let  $a = \sqrt[3]{1+n}$  and  $b = \sqrt[3]{n}$ , then

$$\begin{aligned} \lim_{n \rightarrow +\infty} u_n &= \lim_{n \rightarrow +\infty} \sqrt[3]{1+n} - \sqrt[3]{n} \\ &= \lim_{n \rightarrow +\infty} \frac{(\sqrt[3]{1+n})^3 - (\sqrt[3]{n})^3}{(\sqrt[3]{1+n})^2 + \sqrt[3]{n(1+n)} + (\sqrt[3]{n})^2} \\ &= \lim_{n \rightarrow +\infty} \frac{1}{(\sqrt[3]{1+n})^2 + \sqrt[3]{n(1+n)} + (\sqrt[3]{n})^2} = 0 \end{aligned}$$

Therefore  $u_n$  C.V.

$$7) u_n = \left( \frac{n^2 - n + 3}{n^2 + 3n - 1} \right)^n.$$

Firstly

$$\begin{aligned} \lim_{n \rightarrow +\infty} u_n &= \lim_{n \rightarrow +\infty} \left( \frac{n^2 - n + 3}{n^2 + 3n - 1} \right)^n \\ &= \lim_{n \rightarrow +\infty} \left( 1 - \frac{4n - 4}{n^2 + 3n - 1} \right)^n \quad (\text{using Euclidean division}) \\ &= \lim_{n \rightarrow +\infty} \left( 1 - \frac{4n - 4}{n^2 + 3n - 1} \right)^n \left( \frac{n^2 + 3n - 1}{-4n + 4} \right) \left( \frac{-4n + 4}{n^2 + 3n - 1} \right). \end{aligned}$$

We have  $\lim_{n \rightarrow +\infty} n \left( \frac{-4n + 4}{n^2 + 3n - 1} \right) = -4$ . Moreover, we set  $X = \frac{-4n + 4}{n^2 + 3n - 1}$  to obtain

$$n \rightarrow +\infty \implies X \rightarrow 0.$$

Hence

$$\lim_{n \rightarrow +\infty} u_n = \lim_{X \rightarrow 0} (1 + X)^{\frac{-4}{X}} = \lim_{X \rightarrow 0} e^{\frac{-4 \ln(1+X)}{X}} = e^{-4}.$$

Then,  $u_n$  is C.V.

$$8) u_n = \frac{5 \times 7 \times \cdots \times (2n + 5)}{4 \times 7 \times \cdots \times (3n + 4)}.$$

This type is always treated in the same way;  $u_{n+1}$  must be expressed as a function of  $u_n$ , i.e.,

$$u_{n+1} = \frac{5 \times 7 \times \cdots \times (2n + 5) \times (2n + 7)}{4 \times 7 \times \cdots \times (3n + 4) \times (3n + 7)} = u_n \times \frac{2n + 7}{3n + 7}.$$

If the limit  $\ell$  exists, then it verifies

$$\ell = \ell \times \frac{2}{3} \implies \ell \left( 1 - \frac{2}{3} \right) = 0 \implies \ell = 0.$$

It remains to show that  $u_n$  converges. Clearly,  $u_n > 0$ , i.e.,  $u_n$  is bounded below, and we note

$$\frac{u_{n+1}}{u_n} = \frac{2}{3} < 1.$$

Therefore,  $(u_n)_n$  is decreasing and bounded below, so it converges.

From the above result, the only possible limit is "0".

### Adjacent Sequences

**Exercise 3.** I) Let  $a, b \in \mathbb{R}$ ,  $0 < a \leq b$ . Let the numerical sequences  $(u_n)_n$  and  $(v_n)_n$  be given by

$$\begin{cases} u_0 = a, \\ u_{n+1} = \frac{2u_n + v_n}{3}, \quad \forall n \in \mathbb{N}. \end{cases} \quad \begin{cases} v_0 = b, \\ v_{n+1} = \frac{2v_n + u_n}{3}, \quad \forall n \in \mathbb{N}. \end{cases}$$

1. Calculate  $u_1$  and  $v_1$ .

$$u_1 = \frac{2u_0 + v_0}{3} = \frac{2a + b}{3}, \quad v_1 = \frac{2v_0 + u_0}{3} = \frac{2b + a}{3}.$$

2. Prove that: " $\forall n \in \mathbb{N}$ ,  $u_n \leq u_{n+1} \leq v_{n+1} \leq v_n$ "  $\cdots$   $P(n)$

We will show by induction that the property  $P(n)$  is true for  $n \in \mathbb{N}$ .

Step 01. For  $n = 0$ , we have

$$\begin{aligned} \bullet u_1 &= \frac{2a + b}{3} \geq \frac{2a + a}{3} = a = u_0. \text{ Then } u_1 \geq u_0. \\ \bullet v_1 &= \frac{a + 2b}{3} \leq \frac{b + 2b}{3} = b = v_0. \text{ Then } v_1 \leq v_0. \end{aligned}$$

Moreover,  $u_1 - v_1 = \frac{2a + b - a - 2b}{3} = \frac{a - b}{3} \leq 0$  (because  $a \leq b$ ), i.e.,  $u_1 \leq v_1$ .

Therefore,  $u_0 \leq u_1 \leq v_1 \leq v_0$ . So  $P(0)$  is true.

**Step 02.** Assume that  $P(n)$  is true  $\forall n \in \mathbb{N}$  and show that  $P(n+1)$  is true.

We have

$$u_{n+2} = \frac{2u_{n+1} + v_{n+1}}{3} \geq \frac{2u_{n+1} + u_{n+1}}{3} = u_{n+1},$$

$$v_{n+2} = \frac{2v_{n+1} + u_{n+1}}{3} \leq \frac{2v_{n+1} + v_{n+1}}{3} = v_{n+1},$$

and

$$u_{n+2} - v_{n+2} = \frac{2u_{n+1} + v_{n+1}}{3} - \frac{u_{n+1} + 2v_{n+1}}{3} = \frac{u_{n+1} - v_{n+1}}{3} \leq 0 \text{ (because } u_{n+1} \leq v_{n+1}\text{)}.$$

Consequently,  $u_{n+1} \leq u_{n+2} \leq v_{n+2} \leq v_{n+1}$ , i.e.,  $P(n+1)$  is true, so then  $\forall n \in \mathbb{N}$ ,

$$u_n \leq u_{n+1} \leq v_{n+1} \leq v_n.$$

3. Express  $(v_n - u_n)_n$  in terms of  $(b - a)$ . Deduce that  $(u_n)_n$  and  $(v_n)_n$  are adjacent;

• As  $v_{n+1} - u_{n+1} = \frac{2v_n + u_n - 2u_n - v_n}{3} = \frac{v_n - u_n}{3}$ , the sequence  $(v_n - u_n)_n$  is a geometric sequence of reason  $\frac{1}{3}$ , and so

$$v_n - u_n = \left(\frac{1}{3}\right)^n (v_0 - u_0) = \left(\frac{1}{3}\right)^n (b - a).$$

Given that  $0 < \frac{1}{3} < 1$ , the sequence  $(v_n - u_n)_n$  converges to 0. That is  $\lim_{n \rightarrow +\infty} \left(\frac{1}{3}\right)^n (b - a) = 0$ .

According to the previous question, we have

$$\begin{cases} 1) & u_n \leq u_{n+1} \Leftrightarrow (u_n)_n \text{ is increasing.} \\ 2) & v_{n+1} \leq v_n \Leftrightarrow (v_n)_n \text{ is decreasing.} \\ 3) & \lim_{n \rightarrow +\infty} v_n - u_n = 0. \end{cases}$$

Hence, we deduce that  $(u_n)_n$  and  $(v_n)_n$  are adjacent. They therefore converge to the same limit  $\ell$ .

4. Express  $(v_n + u_n)_n$  in terms of  $(a + b)$ , and set the limit of each sequence  $(u_n)_n$  and  $(v_n)_n$ .

$$v_{n+1} + u_{n+1} = \frac{2v_n + u_n + 2u_n + v_n}{3} = v_n + u_n.$$

Thus, the sequence  $(v_n + u_n)_n$  is constant. Then

$$\forall n \in \mathbb{N}, \quad v_n + u_n = v_0 + u_0 = a + b.$$

5. Determine the limit of  $(u_n)_n$  and  $(v_n)_n$ .

As  $(u_n)_n$  and  $(v_n)_n$  are adjacent, so

$$\lim_{n \rightarrow +\infty} u_n = \lim_{n \rightarrow +\infty} v_n = \ell.$$

Thus

$$\lim_{n \rightarrow +\infty} (u_n + v_n) = 2\ell.$$

In the other side, we have  $v_n + u_n = a + b$ , i.e.,  $\lim_{n \rightarrow +\infty} v_n + u_n = a + b$ . Therefore

$$2\ell = a + b \Rightarrow \ell = \frac{a + b}{2}.$$

**II)** Consider the sequence of general term:  $v_n = 1 - \frac{1}{2} + \frac{1}{3} + \dots + \frac{(-1)^{n+1}}{n}$ ,  $\forall n \in \mathbb{N}^*$ .

► Prove that the two subsequences  $(v_{2n})_n$  and  $(v_{2n+1})_n$  are adjacent, then deduce the nature of  $(v_n)_n$ .  
For every  $n \in \mathbb{N}^*$ , we have  $v_{2n} = 1 - \frac{1}{2} + \dots + \frac{(-1)^{2n-1}}{2n} = 1 - \frac{1}{2} + \dots + \frac{1}{2n-1} - \frac{1}{2n}$ . Then

$$\begin{aligned} v_{2(n+1)} - v_{2n} &= \left(1 - \frac{1}{2} + \dots + \frac{1}{2n+1} - \frac{1}{2n+2}\right) - \left(1 - \frac{1}{2} + \dots + \frac{1}{2n-1} - \frac{1}{2n}\right) \\ &= \frac{1}{2n+1} - \frac{1}{2n+2} = \frac{1}{(2n+1)(2n+2)} > 0. \end{aligned}$$

That is,  $(v_{2n})_n$  is increasing. Furthermore

$$\begin{aligned} v_{2(n+1)+1} - v_{2n+1} &= \left(1 - \frac{1}{2} + \dots - \frac{1}{2n+2} + \frac{1}{2n+3}\right) - \left(1 - \frac{1}{2} + \dots - \frac{1}{2n} + \frac{1}{2n+1}\right) \\ &= \frac{-1}{2n+2} + \frac{1}{2n+3} = \frac{-1}{(2n+2)(2n+3)} < 0. \end{aligned}$$

That is,  $(v_{2n+1})_n$  is decreasing.

Now,  $\lim_{n \rightarrow +\infty} v_{2n} - v_{2n+1} = -\frac{1}{2n+1} \xrightarrow{n \rightarrow +\infty} 0$ . Under the above-obtained results, we deduce that,  $(v_{2n})_n$  and  $(v_{2n+1})_n$  are adjacent sequences.

**Conclusion.** As  $(v_{2n})_n$  and  $(v_{2n+1})_n$  are adjacent, these two sequences are convergent and have the same limit  $\ell$ . Consequently,  $(v_n)_n$  converges to  $\ell$ .

## Divergent Sequences

**Exercise 4.** I) Consider the real sequence  $(u_n)_{n \in \mathbb{N}^*}$  defined as:  $u_n = n\sqrt{n}$ .

$$(u_n)_n \text{ diverges to } \pm \infty \iff \begin{pmatrix} \forall A > 0, \exists n_0 \in \mathbb{N}, \forall n \in \mathbb{N}; n \geq n_0 \Rightarrow u_n > A \\ \forall A > 0, \exists n_0 \in \mathbb{N}, \forall n \in \mathbb{N}; n \geq n_0 \Rightarrow u_n < -A \end{pmatrix}.$$

Explain the definition that corresponds to the limit of  $(u_n)_n$ , such that  $u_n \in (10^6; +\infty)$ , then deduce the values of  $A$  and  $n_0$ .

We have  $u_n \in (10^6; +\infty)$  i.e,  $u_n > 10^6$ , then  $u_n$  is bounded below.

On the other hand,  $u_n = n\sqrt{n}$  is increasing.

So,  $(u_n)_n$  is bounded below and increasing, then,  $(u_n)_n$  is divergent to  $+\infty$ .

Therefore, we use the first definition, by it we conclude:

$$u_n > 10^6 \Rightarrow A = 10^6,$$

and  $n\sqrt{n} > 10^6 \Leftrightarrow (\sqrt{n})^3 > 10^6 \Leftrightarrow n > 10^4$ , it's enough to take  $n_0 = [10^4] + 1 = 10001$ .

► Use the previous definitions to prove each of the following:

- $\lim_{n \rightarrow +\infty} 3^{2n+1} = +\infty$ . Using the definition, we have

$$\begin{aligned} \forall A > 0, \exists n_0 \in \mathbb{N}, \forall n \in \mathbb{N}; n \geq n_0 &\Rightarrow 3^{2n+1} > A \\ &\Rightarrow (2n+1) \ln(3) > \ln(A) \\ &\Rightarrow n > \frac{2 \ln(A)}{2 \ln(3)} - \frac{1}{2}. \end{aligned}$$

Then, it's enough to take  $n_0 = \left\lceil \frac{\ln(A)}{2 \ln(3)} - \frac{1}{2} \right\rceil + 1$ .

- $\lim_{n \rightarrow +\infty} \frac{1}{2}(e^{\frac{1}{n}} - n) = -\infty$ . Using the definition, we have

$$\begin{aligned} \forall A > 0, \exists n_0 \in \mathbb{N}, \forall n \in \mathbb{N}; n \geq n_0 &\Rightarrow \frac{1}{2}(e^{\frac{1}{n}} - n) < -A \\ &\Rightarrow e^{\frac{1}{n}} - n < -2A \\ &\Rightarrow -n < -(2A + e^{\frac{1}{n}}) \\ (0 < \frac{1}{n} \leq 1 \Leftrightarrow 1 < e^{\frac{1}{n}} \leq e) &\Rightarrow -n < -(2A + e) \\ &\Rightarrow n > 2A + e \end{aligned}$$

Then, it's enough to take  $n_0 = [2A + e] + 1$ .

**II) Choose the suitable way (subsequences, comparison test) to show that the below sequences are divergent:**

- 1)  $u_n = \cos\left(\frac{n\pi}{4}\right)$ , we choose the subsequences way:

$$\text{If } n = 4k, k \in \mathbb{N}, \text{ we find } u_{4k} = \cos\left(\frac{4k\pi}{4}\right) = \cos(k\pi) = (-1)^k,$$

since, the subsequence  $(-1)^k$  is divergent, then  $(u_n)_n$  is divergent.

- 2)  $u_n = \left(1 + \frac{1}{n}\right)^{n^2}$ , we choose the comparison test:

Since  $\left(1 + \frac{1}{n}\right)^n$  is a monotonically increasing sequence, therefore  $\left(1 + \frac{1}{n}\right)^n \geq 2$ .

$$u_n = \left(1 + \frac{1}{n}\right)^{n^2} = \left(\left(1 + \frac{1}{n}\right)^n\right)^n \geq 2^n \xrightarrow{n \rightarrow +\infty} +\infty.$$

By comparison test, we deduce  $(u_n)_n$  is divergent to  $+\infty$ .

- 3)  $u_n = \frac{n + (-1)^n n}{n - (-1)^{\frac{n}{2}}}$ , we choose the subsequences way:

If  $n = 2k, k \in \mathbb{N}$ , we get

$$u_{2k} = \frac{2k + 2k}{2k - \frac{2k}{2}} = 4 \text{ is a constant sequence converges to } 4.$$

If  $n = 2k + 1, k \in \mathbb{N}$ , we get

$$u_{2k+1} = \frac{2k + 1 - 2k - 1}{2k + 1 - \frac{2k+1}{2}} = 0 \text{ is a constant sequence converges to } 0.$$

Then,  $\lim_{n \rightarrow +\infty} u_{2k} \neq \lim_{n \rightarrow +\infty} u_{2k+1}$ .

Hence,  $(u_n)_n$  is divergent.

- 4)  $\frac{n! + 3^n}{n - 2^n}$ , we choose the comparison test:

$$\text{The order of growth of the denominator is } 2^n : \frac{n! + 3^n}{n - 2^n} = \frac{\frac{n!}{2^n} + \left(\frac{3}{2}\right)^n}{\frac{n}{2^n} - 1}.$$

$$\text{We have, } n < 2^n \Rightarrow \frac{n}{2^n} - 1 < 0 \Rightarrow \frac{1}{\frac{n}{2^n} - 1} < 0, \text{ and } \frac{n}{2^n} \xrightarrow{n \rightarrow +\infty} 0. \quad (*)$$

On the other hand, we have

$$\begin{aligned} \frac{n!}{2^n} + \left(\frac{3}{2}\right)^n &> \frac{n}{2^n} + \left(\frac{3}{2}\right)^n \\ (*) \Downarrow \\ u_n &< \frac{\frac{n}{2^n} + \left(\frac{3}{2}\right)^n}{\frac{n}{2^n} - 1} \xrightarrow{n \rightarrow +\infty} -\infty. \end{aligned}$$

By comparison test, we deduce  $(u_n)_n$  is divergent to  $-\infty$ .

## Cauchy Sequences

**Exercise 5.** I) Consider the real sequence  $(u_n)_{n \in \mathbb{N}^*}$ , such that:

$$|u_{n+1} - u_n| \leq k|u_n - u_{n-1}|, \quad n \in \mathbb{N}^*, \quad k \in (0; 1).$$

I) Show that:  $\forall n \in \mathbb{N}^*, |u_{n+1} - u_n| \leq k^{n-1}|u_2 - u_1|$ .

According to the above inequality, we have

$$\begin{aligned} |u_{n+1} - u_n| &\leq k|u_n - u_{n-1}| \\ &\leq k(k|u_{n-1} - u_{n-2}|) \\ &\leq kk(k|u_{n-2} - u_{n-3}|) \\ &\vdots \\ &\leq \overbrace{kk \cdots k}^{(n-1) \text{ times}} |u_2 - u_1| = k^{n-1}|u_2 - u_1|. \end{aligned}$$

2) Prove that:  $\forall p, q \in \mathbb{N}^*, q < p$ , we have  $|u_p - u_q| \leq \frac{k^{q-1}}{1-k}|u_2 - u_1|$ .

According to the previous question, we have

$$\begin{aligned} |u_p - u_q| &= |u_p - u_{p-1} + u_{p-1} - u_{p-2} + u_{p-2} \cdots + u_{q-1} - u_q| \\ &\leq |u_p - u_{p-1}| + |u_{p-1} - u_{p-2}| + \cdots + |u_{q-1} - u_q| \\ &\leq k^{p-2}|u_2 - u_1| + k^{p-3}|u_2 - u_1| + \cdots + k^{q-1}|u_2 - u_1| \\ &= (k^{p-2} + k^{p-3} + \cdots + k^{q-1})|u_2 - u_1| \\ &= k^{q-1} (k^{p-(q+1)} + k^{p-(q+2)} + \cdots + 1) |u_2 - u_1| \\ &\sum_{i=0}^{p-q-1} k^i \quad \begin{array}{l} \text{is a geometric sequence} \\ \text{of reason } k \end{array} = k^{q-1} \left( \sum_{i=0}^{p-q-1} k^i \right) |u_2 - u_1| \\ &= k^{q-1} \left( \frac{1 - k^{p-q}}{1 - k} \right) |u_2 - u_1| \\ &= \frac{k^{q-1}}{1 - k} (1 - k^{p-q}) |u_2 - u_1|, \quad 1 - k^{p-q} < 1 \\ &\leq \frac{k^{q-1}}{1 - k} |u_2 - u_1|, \end{aligned}$$

3) Deduce the nature of  $(u_n)_n$ . Applying the definition, we have

$$\begin{aligned} \forall \varepsilon > 0, \exists n_0 \in \mathbb{N}, \forall p, q \in \mathbb{N}; p \geq n_0, q \geq n_0 &\Rightarrow |u_p - u_q| < \varepsilon \\ |u_p - u_q| < \varepsilon &\Rightarrow \frac{k^{q-1}}{1 - k} |u_2 - u_1| < \varepsilon \\ &\Rightarrow (q - 1) \ln(k) < \ln \left( \frac{(1 - k)\varepsilon}{|u_2 - u_1|} \right) \\ &\Rightarrow q > \ln \left( \frac{(1 - k)\varepsilon}{|u_2 - u_1|} \right) \times \frac{1}{\ln(k)} + 1. \end{aligned}$$

$$\text{Then, it's enough to take } n_0 = \left\lceil \ln \left( \frac{(1 - k)\varepsilon}{|u_2 - u_1|} \right) \times \frac{1}{\ln(k)} + 1 \right\rceil + 1.$$

Consequently,  $(u_n)_n$  is a Cauchy sequence, so it is convergent.

II) In view of the Cauchy criterion, determine the nature of the sequences  $(u_n)_n$  defined by:

I)  $u_n = \sum_{k=1}^n \frac{1}{\sqrt{k}} = 1 + \frac{1}{\sqrt{2}} + \cdots + \frac{1}{\sqrt{n}}$ . Using the Cauchy criterion:

$$\forall \varepsilon > 0, \exists n_0 \in \mathbb{N}^*, \forall p, q \in \mathbb{N}^*; p > q, p \geq n_0, q \geq n_0 \Rightarrow |u_p - u_q| < \varepsilon.$$



$$\begin{aligned}
|u_p - u_q| &= \left| 1 + \frac{1}{\sqrt{2}} + \cdots + \frac{1}{\sqrt{q}} + \frac{1}{\sqrt{q+1}} + \cdots + \frac{1}{\sqrt{p}} - \left( 1 + \frac{1}{\sqrt{2}} + \cdots + \frac{1}{\sqrt{q}} \right) \right| \\
&= \left| \frac{1}{\sqrt{q+1}} + \frac{1}{\sqrt{q+2}} + \cdots + \frac{1}{\sqrt{p}} \right|.
\end{aligned}$$

If we take  $p = 2n > q = n$ , we get

$$\begin{aligned}
|u_{2n} - u_n| &= \left| \frac{1}{\sqrt{n+1}} + \frac{1}{\sqrt{n+2}} + \cdots + \frac{1}{\sqrt{2n}} \right| \\
&\geq \left| \frac{n}{\sqrt{2n}} \right| = \sqrt{\frac{n}{2}} \geq \frac{1}{\sqrt{2}}.
\end{aligned}$$

Therefore,  $\exists \varepsilon = \frac{1}{\sqrt{2}} > 0$ ,  $\forall n_0 \in \mathbb{N}^*$ ,  $\exists p = 2n \wedge \exists q = n$ ,  $\exists p \geq n_0 \wedge q \geq n_0 \wedge |u_p - u_q| \geq \varepsilon$ .

Thus,  $(u_n)_n$  isn't Cauchy and deduce that  $(u_n)_n$  is divergent.

2)  $u_n = \sum_{k=1}^n \frac{\sin k}{2^k} = \frac{\sin(1)}{2} + \frac{\sin(2)}{2^2} + \cdots + \frac{\sin(n)}{2^n}$ . Using the Cauchy criterion:

$$\forall \varepsilon > 0, \exists n_0 \in \mathbb{N}^*, \forall p, q \in \mathbb{N}^*; p > q, p \geq n_0, q \geq n_0 \Rightarrow |u_p - u_q| < \varepsilon.$$

$$\begin{aligned}
|u_p - u_q| &= \left| \sum_{k=1}^p \frac{\sin k}{2^k} - \sum_{k=1}^q \frac{\sin k}{2^k} \right| = \left| \sum_{k=q+1}^p \frac{\sin k}{2^k} \right| \\
&\leq \sum_{k=q+1}^p \frac{1}{2^k} = \frac{1}{2^{q+1}} + \frac{1}{2^{q+2}} + \cdots + \frac{1}{2^p} \\
&= \frac{1}{2^{q+1}} \left( 1 + \frac{1}{2} + \frac{1}{2^2} + \cdots + \frac{1}{2^{p-q-1}} \right) \text{ is a geometric sequence of reason } 1/2 \\
&= \frac{1}{2^{q+1}} \left( 1 \times \frac{1 - \left(\frac{1}{2}\right)^{p-q}}{1 - \frac{1}{2}} \right) = \frac{1}{2^q} \left( 1 - \left(\frac{1}{2}\right)^{p-q} \right) \\
&\leq \frac{1}{2^q} < \varepsilon \Rightarrow 2^q > \frac{1}{\varepsilon} \Rightarrow q > \frac{\ln(1/\varepsilon)}{\ln(2)}.
\end{aligned}$$

Then, it's enough to take  $n_0 = \left\lceil \frac{\ln(1/\varepsilon)}{\ln(2)} \right\rceil + 1 \in \mathbb{N}$ , therefore  $(u_n)_n$  is convergent.

## Recurrence Sequences

**Exercise 6.** Let the sequence  $(u_n)_n$  be recursively defined by:

$$\begin{cases} u_0 \in \mathbb{R}, \\ u_{n+1} = \frac{u_n}{(u_n)^2 + 1}, \quad n \in \mathbb{N}. \end{cases}$$

1. We set  $u_0 = \alpha$ . Determine  $\alpha$ , such that the sequence  $(u_n)_n$  is zero.

$$\left( (u_n)_n \text{ is zero} \iff u_0 = u_1 = u_2 = \cdots = u_n = 0 \right) \Rightarrow \left( \alpha = 0 \text{ because } u_0 = \alpha \right).$$

2. For  $u_n > 0$ .

(a) Prove that: " $\forall n \in \mathbb{N}, u_n > 0$ ". By induction, we have

**Step 01.** For  $n = 0$ , we get from the data  $u_0 > 0$ .

**Step 02.** Suppose that  $u_n > 0$ ,  $\forall n \in \mathbb{N}$  is true and we must show that  $u_{n+1} > 0$ ,  $\forall n \in \mathbb{N}$ .

The condition  $u_n > 0$  give us  $\frac{1}{(u_n)^2 + 1} > 0$ , and so  $u_{n+1} = \frac{u_n}{(u_n)^2 + 1} > 0$ .

Therefore; by induction,  $\forall n \in \mathbb{N}, u_n > 0$ .

(b) Show that  $(u_n)_n$  is strictly decreasing.

We have  $u_n > 0$  and  $\frac{1}{(u_n)^2 + 1} < 1 \iff \frac{u_n}{(u_n)^2 + 1} < u_n \iff u_{n+1} < u_n$ .

Then  $(u_n)_n$  is strictly decreasing.

(c) Deduce that  $(u_n)_n$  is convergent and compute its limit.

The sequence  $(u_n)_n$  is strictly decreasing and bounded below by 0, then  $(u_n)_n$  is C.V.

On the other hand, we have  $u_{n+1} = f(u_n)$ , where  $f(x) = \frac{x}{x^2 + 1}$  is a continuous function. Then

$$f(\ell) = \ell \iff \ell = \frac{\ell}{\ell^2 + 1} \iff \ell^2 = 0 \iff \ell = 0.$$

3. For  $u_n < 0$ . (In the same previous way).

4. Determine sup, inf, max, and min if they exist in the set  $E = \{|u_n|, n \in \mathbb{N}\}$ .

• Si  $u_0 = 0$  then  $E = \{u_n = 0, \forall n \in \mathbb{N}\} = \{0\}$ . Then  $\sup(E) = \max(E) = \inf(E) = \min(E) = 0$ .

• Si  $u_n > 0$  then  $E = \{u_n, n \in \mathbb{N}\}$ .

Here, the sequence  $(u_n)_n$  is decreasing and convergent to 0. Thus

$$\inf(E) = \lim_{n \rightarrow +\infty} u_n = 0 \notin E \implies \min(E) \text{ does not exist,}$$

and

$$\sup(E) = \max(E) = u_0 \in E \text{ (because } u_0 > u_1 > u_2 > \dots \text{)}.$$

• Si  $u_n < 0$ , then  $E = \{-u_n, n \in \mathbb{N}\}$ .

In this case, we have  $(u_n)_n$  is increasing and convergent to 0. Thus

$$\inf\{u_n, n \in \mathbb{N}\} = u_0 \text{ (because } u_0 < u_1 < u_2 < \dots \text{)},$$

and

$$\sup\{u_n, n \in \mathbb{N}\} = \lim_{n \rightarrow +\infty} u_n = 0.$$

As a consequence,  $(-u_n)_n$  is decreasing and convergent to 0, that is

$$\sup(E) = \max(E) = -u_0 \in E \text{ and } \inf(E) = \lim_{n \rightarrow +\infty} -u_n = 0 \notin E, \text{ i.e., } \min(E) \nexists.$$

Finally, we can summarize the three cases by:

1. if  $u_0 = 0$  :

$$\sup(E) = \max(E) = \inf(E) = \min(E) = 0.$$

2. if  $u_0 \neq 0$  :

$$\sup(E) = \max(E) = |u_0| \text{ and } \inf(E) = 0, \text{ with } \min(E) \nexists.$$